WithTop and WithBot

Discretion/FinExcept/Option.lean
@@ -145,11 +145,242 @@ theorem get_cons_tail (h : y ≠ x) (hy : y ∈ f.support)
 
 end GetSet
 
--- TODO: bot theorems
+section WithTop
 
--- TODO: top theorems
+variable [DecidableEq α] [DecidableEq M]
+  {f g : α →ᶠ[{⊤}] (WithTop M)} {x y : α} {a : M}
 
--- TODO: default theorems?
+theorem not_mem_support_iff_top : x ∉ f.support ↔ f x = ⊤ := not_mem_support_iff
+
+theorem mem_support_iff_ne_top : x ∈ f.support ↔ f x ≠ ⊤ := by simp [not_mem_support_iff_top]
+
+theorem mem_support_of_eq_coe_top : f x = ↑a → x ∈ f.support := mem_support_of_eq_coe
+
+theorem mem_support_of_coe_eq_top : ↑a = f x → x ∈ f.support := mem_support_of_coe_eq
+
+/-- Get an element in the support of `f` -/
+def untop (f : α →ᶠ[{⊤}] (WithTop M)) (x : α) (hx : x ∈ f.support) : M
+  := (f x).untop (mem_support_iff_ne_top.mp hx)
+
+theorem untop_eq_get {hx : x ∈ f.support} : f.untop x hx = f.get x hx := by
+  simp only [untop, get, WithTop.untop, Option.get]
+  split
+  rename_i h _
+  split
+  rename_i h' _
+  cases h.symm.trans h'
+  rfl
+
+@[simp]
+theorem untop_eq (hx : x ∈ f.support) : ↑(f.untop x hx) = f x := by simp [untop]
+
+theorem untop_eq_of_eq_coe (h : f x = ↑a) : f.untop x (mem_support_of_eq_coe h) = a := by
+  simp [untop, h]
+
+theorem untop_eq_of_coe_eq (h : ↑a = f x) : f.untop x (mem_support_of_coe_eq h) = a := by
+  simp [untop, <-h]
+
+theorem untop_eq_iff_eq_at (hx : x ∈ f.support) (hy : y ∈ f.support)
+  : f.untop x hx = f.untop y hy ↔ f x = f y
+  := untop_eq_get.symm ▸ untop_eq_get.symm ▸ get_eq_iff_eq_at hx hy
+
+/-- This is the same as `f.update x ↑a`, but with nicer defeqs for the support -/
+def cons_top (x : α) (a : M) (f : α →ᶠ[{⊤}] (WithTop M)) : α →ᶠ[{⊤}] (WithTop M) where
+  support := insert x f.support
+  toFun := Function.update f x a
+  mem_support_toFun y := by simp only [Function.update]; aesop
+
+theorem cons_top_eq_cons : @cons_top = @cons := rfl
+
+theorem cons_top_apply : (f.cons_top x a) y = if y = x then ↑a else f y := cons_apply
+
+theorem cons_top_head : (f.cons_top x a) x = ↑a := cons_head
+
+theorem cons_top_tail : y ≠ x → (f.cons_top x a) y = f y := cons_tail
+
+@[simp, norm_cast]
+theorem coe_cons_top : (f.cons_top x a : α → WithTop M) = Function.update f x a := rfl
+
+@[simp]
+theorem top_cons_top : cons_top x a ⊤ = single ⊤ x ↑a := by
+  ext
+  rw [single_eq_update]
+  rfl
+
+@[simp]
+theorem default_cons_top : cons_top x a default = single ⊤ x ↑a := top_cons_top
+
+theorem support_cons_top :
+    support (f.cons_top x a) = insert x f.support := rfl
+
+theorem cons_top_eq_update (x : α) (a : M) (f : α →ᶠ[{⊤}] (WithTop M))
+  : cons_top x a f = f.update x a :=
+  rfl
+
+@[simp]
+theorem cons_top_eq_self (h : x ∈ f.support)
+  : f.cons_top x (f.untop x h) = f := by simp [cons_top_eq_update]
+
+theorem cons_top_comm (f : α →ᶠ[{none}] (Option M)) (h : x ≠ y) (a b : M) :
+  cons_top x a (cons_top y b f) = cons_top y b (cons_top x a f)
+  := by simp only [cons_top_eq_update, f.update_comm h]
+
+@[simp]
+theorem cons_top_idem (x : α) (a : M) (f : α →ᶠ[{none}] (Option M))
+  : cons_top x a (cons_top x a f) = cons_top x a f :=
+  by simp only [cons_top_eq_update, f.update_idem]
+
+theorem eq_at_of_cons_top_eq_self (h : cons_top x a f = f) : a = f x := by
+  have h : cons_top x a f x = f x := by rw [h];
+  simp only [cons_top_apply, ↓reduceIte] at h
+  rw [h]
+
+theorem cons_top_eq_self_of_eq_at (h : a = f x) : cons_top x a f = f := by
+  ext
+  simp only [cons_top_apply]
+  split <;> simp [*]
+
+@[simp]
+theorem cons_top_eq_self_iff : cons_top x a f = f ↔ a = f x := cons_eq_self_iff
+
+@[simp]
+theorem eq_self_cons_top_iff : f = cons_top x a f ↔ f x = a := eq_self_cons_iff
+
+theorem ne_cons_top_self_iff : f ≠ cons_top x a f ↔ f x ≠ a := ne_cons_self_iff
+
+theorem cons_top_ne_self_iff : cons_top x a f ≠ f ↔ ↑a ≠ f x := cons_ne_self_iff
+
+theorem mem_support_cons_top : x ∈ (cons_top x a f).support := mem_support_cons
+
+theorem mem_support_cons_top_of_mem_support : y ∈ f.support → y ∈ (cons_top x a f).support
+  := mem_support_cons_of_mem_support
+
+theorem mem_support_of_cons_top_eq (h : cons_top x a f = g) : x ∈ g.support := h ▸ mem_support_cons
+
+theorem mem_support_of_eq_cons_top : g = cons_top x a f → x ∈ g.support
+  := mem_support_of_eq_cons
+
+theorem cons_top_eq_iff : cons_top x a f = g ↔ g x = a ∧ ∀y, y ≠ x -> f y = g y := cons_eq_iff
+
+theorem eq_cons_top_iff : g = cons x a f ↔ a = g x ∧ ∀y, y ≠ x -> g y = f y := eq_cons_iff
+
+@[simp]
+theorem untop_cons_head : (cons_top x a f).untop x (mem_support_cons) = a := by simp [untop]
+
+theorem untop_cons_tail (h : y ≠ x) (hy : y ∈ f.support)
+  : (cons_top x a f).untop y (mem_support_cons_of_mem_support hy) = f.untop y hy
+  := by simp [untop, h]
+
+end WithTop
+
+section WithBot
+
+variable [DecidableEq α] [DecidableEq M]
+  {f g : α →ᶠ[{⊥}] (WithBot M)} {x y : α} {a : M}
+
+theorem not_mem_support_iff_bot : x ∉ f.support ↔ f x = ⊥ := not_mem_support_iff
+
+theorem mem_support_iff_ne_bot : x ∈ f.support ↔ f x ≠ ⊥ := by simp [not_mem_support_iff_bot]
+
+theorem mem_support_of_eq_coe_bot : f x = ↑a → x ∈ f.support := mem_support_of_eq_coe
+
+theorem mem_support_of_coe_eq_bot : ↑a = f x → x ∈ f.support := mem_support_of_coe_eq
+
+/-- Get an element in the support of `f` -/
+def unbot (f : α →ᶠ[{⊥}] (WithBot M)) (x : α) (hx : x ∈ f.support) : M
+  := (f x).unbot (mem_support_iff_ne_bot.mp hx)
+
+theorem unbot_eq_get {hx : x ∈ f.support} : f.unbot x hx = f.get x hx := untop_eq_get
+
+@[simp]
+theorem unbot_eq (hx : x ∈ f.support) : ↑(f.unbot x hx) = f x := untop_eq hx
+
+theorem unbot_eq_of_eq_coe (h : f x = ↑a) : f.unbot x (mem_support_of_eq_coe h) = a
+  := untop_eq_of_eq_coe h
+
+theorem unbot_eq_of_coe_eq (h : ↑a = f x) : f.unbot x (mem_support_of_coe_eq h) = a
+  := untop_eq_of_coe_eq h
+
+theorem unbot_eq_iff_eq_at (hx : x ∈ f.support) (hy : y ∈ f.support)
+  : f.unbot x hx = f.unbot y hy ↔ f x = f y
+  := untop_eq_iff_eq_at hx hy
+
+/-- This is the same as `f.update x ↑a`, but with nicer defeqs for the support -/
+def cons_bot (x : α) (a : M) (f : α →ᶠ[{⊥}] (WithBot M)) : α →ᶠ[{⊥}] (WithBot M) where
+  support := insert x f.support
+  toFun := Function.update f x a
+  mem_support_toFun y := by simp only [Function.update]; aesop
+
+theorem cons_bot_apply : (f.cons_bot x a) y = if y = x then ↑a else f y := cons_apply
+
+theorem cons_bot_head : (f.cons_bot x a) x = ↑a := cons_head
+
+theorem cons_bot_tail : y ≠ x → (f.cons_bot x a) y = f y := cons_tail
+
+@[simp, norm_cast]
+theorem coe_cons_bot : (f.cons_bot x a : α → WithBot M) = Function.update f x a := rfl
+
+@[simp]
+theorem bot_cons_bot : cons_bot x a ⊥ = single ⊥ x ↑a := top_cons_top
+
+@[simp]
+theorem default_cons_bot : cons_bot x a default = single ⊥ x ↑a := bot_cons_bot
+
+theorem support_cons_bot :
+    support (f.cons_bot x a) = insert x f.support := rfl
+
+theorem cons_bot_eq_update (x : α) (a : M) (f : α →ᶠ[{⊥}] (WithBot M))
+  : cons_bot x a f = f.update x a :=
+  rfl
+
+@[simp]
+theorem cons_bot_eq_self (h : x ∈ f.support) : f.cons_bot x (f.unbot x h) = f := cons_top_eq_self h
+
+theorem cons_bot_comm (f : α →ᶠ[{none}] (Option M)) (h : x ≠ y) (a b : M) :
+  cons_bot x a (cons_bot y b f) = cons_bot y b (cons_bot x a f) := cons_top_comm f h a b
+
+@[simp]
+theorem cons_bot_idem (x : α) (a : M) (f : α →ᶠ[{none}] (Option M))
+  : cons_bot x a (cons_bot x a f) = cons_bot x a f := cons_top_idem x a f
+
+theorem eq_at_of_cons_bot_eq_self (h : cons_bot x a f = f) : a = f x := eq_at_of_cons_top_eq_self h
+
+theorem cons_bot_eq_self_of_eq_at (h : a = f x) : cons_bot x a f = f := cons_top_eq_self_of_eq_at h
+
+@[simp]
+theorem cons_bot_eq_self_iff : cons_bot x a f = f ↔ a = f x := cons_eq_self_iff
+
+@[simp]
+theorem eq_self_cons_bot_iff : f = cons_bot x a f ↔ f x = a := eq_self_cons_iff
+
+theorem ne_cons_bot_self_iff : f ≠ cons_bot x a f ↔ f x ≠ a := ne_cons_self_iff
+
+theorem cons_bot_ne_self_iff : cons_bot x a f ≠ f ↔ ↑a ≠ f x := cons_ne_self_iff
+
+theorem mem_support_cons_bot : x ∈ (cons_bot x a f).support := mem_support_cons
+
+theorem mem_support_cons_bot_of_mem_support : y ∈ f.support → y ∈ (cons_bot x a f).support
+  := mem_support_cons_of_mem_support
+
+theorem mem_support_of_cons_bot_eq (h : cons_bot x a f = g) : x ∈ g.support := h ▸ mem_support_cons
+
+theorem mem_support_of_eq_cons_bot : g = cons_bot x a f → x ∈ g.support
+  := mem_support_of_eq_cons
+
+theorem cons_bot_eq_iff : cons_bot x a f = g ↔ g x = a ∧ ∀y, y ≠ x -> f y = g y := cons_eq_iff
+
+theorem eq_cons_bot_iff : g = cons x a f ↔ a = g x ∧ ∀y, y ≠ x -> g y = f y := eq_cons_iff
+
+@[simp]
+theorem unbot_cons_head : (cons_bot x a f).unbot x (mem_support_cons) = a := by simp [unbot]
+
+theorem unbot_cons_tail (h : y ≠ x) (hy : y ∈ f.support)
+  : (cons_bot x a f).unbot y (mem_support_cons_of_mem_support hy) = f.unbot y hy
+  := by simp [unbot, h]
+
+end WithBot
+
+-- TODO: default theorems
 
 -- TODO: injectivity and monotonicity theorems
 
